theories/tree_borrows/steps_access.v
@@ -226,29 +226,5 @@ Proof.
   - exfalso. subst l'. by rewrite EqD in EqN.
 Qed.
 
-Lemma trees_deallocate_isSome trs cids tg blk m sz :
-  is_Some (apply_within_trees (memory_deallocate cids tg (m, sz)) blk trs) ->
-  exists tr, trs !! blk = Some tr /\ is_Some (memory_deallocate cids tg (m, sz) tr).
-Proof.
-  unfold apply_within_trees. destruct (trs !! blk); simpl; [|intro H; inversion H; inversion H0].
-  exists t. destruct (memory_deallocate cids tg (m, sz) t); simpl; [|inversion H; inversion H0].
-  auto.
-Qed.
-
-
-
-
-Lemma tree_dealloc_Some tr fn cids tg range dyn_rel :
-  is_Some (tree_apply_access fn cids tg range tr dyn_rel) ->
-  every_node (fun it => is_Some (fn cids (if dyn_rel (itag it) tg then AccessChild else AccessForeign) range it)) tr.
-Proof.
-  unfold tree_apply_access.
-  intro Success. rewrite join_success_condition in Success.
-  rewrite every_node_eqv_universal.
-  rewrite every_node_map in Success.
-  rewrite every_node_eqv_universal in Success.
-  unfold compose in Success; apply Success.
-Qed.
-
 
 
